Proving the block execution of the reduce template

Examples/Reduce_opt_skel.v
@@ -14,21 +14,22 @@ Qed.
 
 Ltac simplify :=
   unfold vars2es, tarr_idx, vs2es in *;
-  repeat (simpl in *; subst; lazymatch goal with
+  repeat (simpl in *; substs; lazymatch goal with
           | [|- In _ (map _ _) -> _] =>
-            rewrite in_map_iff; intros [? [? ?]]; subst
+            rewrite in_map_iff; intros [? [? ?]]; substs
           | [H:In _ (map _ _) |-_] =>
-            rewrite in_map_iff in H; destruct H as [? [? H]]; subst
+            rewrite in_map_iff in H; destruct H as [? [? H]]; substs
           | [|- indeE _ _] => apply indeE_fv
           | [|- indelE _ _] => apply indelE_fv
-          | [H : _ \/ False|-_] =>destruct H as [H|[]];subst
+          | [H : _ \/ False|-_] =>destruct H as [H|[]];substs
           | [H : _ \/ _ |-_] =>destruct H as [?|H]
           | [|- ~(_ \/ _)] => intros [?|?]
           | [|- context [In _ (_ ++ _)]] => rewrite in_app_iff
+          | [H : context [In _ (_ ++ _)] |- _] => rewrite in_app_iff in H
           | [|- forall _, _] => intros ?
           | [H : In _ (locals _ _) |- _] => apply locals_pref in H
           | [H : In _ (nseq _ _) |- _] => apply nseq_in in H
-          | [H : prefix _ _ = true |- _] => apply prefix_ex in H as [? ?]; subst
+          | [H : prefix _ _ = true |- _] => apply prefix_ex in H as [? ?]; substs
           | [|- disjoint_list (locals _ _)] => apply locals_disjoint_ls
           | [|- context [length (locals _ _)]] => rewrite locals_length
           | [H :context [length (locals _ _)]|- _] => rewrite locals_length in H
@@ -36,7 +37,7 @@ Ltac simplify :=
           | [|- context [length (vars2es _)]] => unfold vars2es; rewrite map_length
           | [H :context [In _ (vars2es _)]|- _] =>
             unfold vars2es in *; rewrite in_map_iff in H;
-            destruct H as [? [? H]]; subst
+            destruct H as [? [? H]]; substs
           | [|- context [In _ (vars2es _)]] => unfold vars2es; rewrite in_map_iff
           | [|- Forall _ _] => rewrite Forall_forall; intros
           | [|- indeE _ _] => apply indeE_fv
@@ -49,7 +50,7 @@ Ltac simplify :=
           | [|- context [length (map _ _)]] => rewrite map_length
           | [H : context [length (map _ _)] |- _] => rewrite map_length in H
           | [|- ~_] => intros ?
-          end; simpl in *; subst).
+          end; simpl in *; try substs).
 
 Section Sum_of.
   Variable T : Type.
@@ -204,8 +205,11 @@ Section Reduce.
 
   (* initial value of the output array *)
   Variable fout : nat -> list val.
-
+  (* the top address of the output array *)
+  Variable out : list Z.
+  Hypothesis out_wf : length out = dim.
   Definition Outs := locals "Out" dim.
+  Notation Outs' := (vars2es Outs). 
   
   Open Scope string_scope.
   
@@ -1545,61 +1549,22 @@ Section Reduce.
 
   Definition sh_decl := map (fun sv => (sv, ntrd)) (locals "sdata" dim).
 
-  Ltac simplify :=
-    unfold vars2es, tarr_idx, vs2es in *;
-    repeat (simpl in *; substs; lazymatch goal with
-            | [|- In _ (map _ _) -> _] =>
-              rewrite in_map_iff; intros [? [? ?]]; substs
-            | [H:In _ (map _ _) |-_] =>
-              rewrite in_map_iff in H; destruct H as [? [? H]]; substs
-            | [|- indeE _ _] => apply indeE_fv
-            | [|- indelE _ _] => apply indelE_fv
-            | [H : _ \/ False|-_] =>destruct H as [H|[]];substs
-            | [H : _ \/ _ |-_] =>destruct H as [?|H]
-            | [|- ~(_ \/ _)] => intros [?|?]
-            | [|- context [In _ (_ ++ _)]] => rewrite in_app_iff
-            | [H : context [In _ (_ ++ _)] |- _] => rewrite in_app_iff in H
-            | [|- forall _, _] => intros ?
-            | [H : In _ (locals _ _) |- _] => apply locals_pref in H
-            | [H : In _ (nseq _ _) |- _] => apply nseq_in in H
-            | [H : prefix _ _ = true |- _] => apply prefix_ex in H as [? ?]; substs
-            | [|- disjoint_list (locals _ _)] => apply locals_disjoint_ls
-            | [|- context [length (locals _ _)]] => rewrite locals_length
-            | [H :context [length (locals _ _)]|- _] => rewrite locals_length in H
-            | [H :context [length (vars2es _)]|- _] => unfold vars2es in *; rewrite map_length
-            | [|- context [length (vars2es _)]] => unfold vars2es; rewrite map_length
-            | [H :context [In _ (vars2es _)]|- _] =>
-              unfold vars2es in *; rewrite in_map_iff in H;
-              destruct H as [? [? H]]; substs
-            | [|- context [In _ (vars2es _)]] => unfold vars2es; rewrite in_map_iff
-            | [|- Forall _ _] => rewrite Forall_forall; intros
-            | [|- indeE _ _] => apply indeE_fv
-            | [|- indelE _ _] => apply indelE_fv
-            | [|- indeB _ _] => apply indeB_fv
-            | [H : context [var_of_str ?x] |- _] => destruct x
-            | [|- inde (_ ==t _) _] => apply inde_eq_tup
-            | [|- inde (_ -->l (_, _)) _] => apply inde_is_tup
-            | [|- inde (is_tuple_array_p _ _ _ _ _) _] => apply inde_is_tup_arr
-            | [|- context [length (map _ _)]] => rewrite map_length
-            | [H : context [length (map _ _)] |- _] => rewrite map_length in H
-            | [|- ~_] => intros ?
-            end; simpl in *; try substs).
-
-  Notation Outs' := (vars2es Outs). 
 
   Theorem reduce_ok_th g :
     (forall i, i < l -> get_den (Zn i) (g i)) ->
     CSL (BS' g) i
-     (!(tid === Zn (nf i)) ** !(bid === Zn (nf j)) ** !(sh === Zn l) **
+     (!(tid === Zn (nf i)) ** !(bid === Zn (nf j)) ** !(sh === Zn l) ** !(Outs' ==t out) **
       (sdata' +ol Zn (nf i) -->l (1, vs2es vi_ini)) **
       input_spec env env_den (perm_n nt_gr) **
-      if Nat.eq_dec (nf i) 0 then map Gl Outs' +ol Zn (nf j) -->l (1, vs2es (fout (nf j)))
-      else emp)
+      if Nat.eq_dec (nf i) 0 then map Gl Outs' +ol Zn (nf j) -->l (1, vs2es (fout (nf j))) else emp)
         
      mkFoldAll
      
      ((if Nat.eq_dec (nf i) 0 then sh_spec sh_decl else emp) **
-      (if Nat.eq_dec (nf i) 0 then map Gl Outs' +ol Zn (nf j) -->l (1, vs2es (f (Nat.min (l - nf j * ntrd) ntrd) (f_seq g) e_b 0)) else emp) **
+      (if Nat.eq_dec (nf i) 0 then
+         map Gl (vs2es out) +ol Zn (nf j) -->l
+             (1, vs2es (f (Nat.min (l - nf j * ntrd) ntrd) (f_seq g) e_b 0))
+       else emp) **
       input_spec' env_den (perm_n nt_gr)).
   Proof.
     intros Hg.
@@ -1687,6 +1652,8 @@ Section Reduce.
           try omega; simpl in *; simplify; simpl; try congruence.
         unfold Outs in *.
         forwards * : reduce_writes; destruct e_b; 
+          try omega; simpl in *; simplify; simpl; try congruence.
+        unfold Outs in *; forwards * : reduce_writes; destruct e_b; 
           try omega; simpl in *; simplify; simpl; try congruence. } }
     hoare_forward; eauto using rule_skip.
     { eapply rule_seq.
@@ -1695,7 +1662,7 @@ Section Reduce.
         { intros s h H.
           sep_normal_in H; sep_split_in H.
           change_in H.
-          { destruct Nat.eq_dec; [|unfold_pures; try omega].
+          { destruct Nat.eq_dec; [|clear HP6; unfold_pures; try omega].
             sep_rewrite_in (is_array_tup_unfold sdata' 0) H; try omega.
             Focus 2. {
               intros; unfold vars2es; rewrite f_length, !map_length, locals_length; eauto.
@@ -1710,7 +1677,7 @@ Section Reduce.
             eauto. }
           clear  HP0 HP1 HP3 HP4 HP5; sep_combine_in H.
           evar (P : assn);
-            assert (((sdata' +ol 0%Z -->l (1, vs2es (f (min (l - ` (Fin.to_nat j) * ntrd) ntrd) (f_seq g) e_b 0))) ** P) s h). 
+            assert (((sdata' +ol 0%Z -->l (1, vs2es (f (min (l - nf j * ntrd) ntrd) (f_seq g) e_b 0))) ** P) s h). 
           { sep_normal_in H; sep_cancel; unfold P; eauto. }
           unfold P in *; eauto. } Unfocus.
         
@@ -1725,9 +1692,8 @@ Section Reduce.
             congruence.
           + rewrite length_nseq; auto. 
         - rewrite gen_read_writes; [|unfold vars2es; rewrite map_length, !locals_length; eauto].
-          prove_inde; simplify; simpl in *; try congruence.
-          apply inde_input_spec; simplify; simpl; congruence.
-          unfold Outs in *; simplify; congruence. }
+          unfold Outs in *; prove_inde; simplify; simpl in *; try congruence.
+          apply inde_input_spec; simplify; simpl; congruence. }
       
       { eapply Hbackward.
         Focus 2. {
@@ -1791,20 +1757,19 @@ Section Reduce.
         { unfold vs2es, vars2es, Outs; rewrite !map_length, !locals_length; auto. }
         rewrite writes_var_gen_write; apply inde_nil. } }
     intros s h [H | H]; sep_normal_in H; sep_split_in H; unfold_pures.
-    - destruct Nat.eq_dec; try omega.
+    - destruct Nat.eq_dec; [|clear HP2; unfold_pures; omega].
       assert (Heq : (bid === Zn (nf j)) s (emp_ph loc)) by (unfold_conn; simpl; eauto).
       sep_rewrite_in mps_eq1_tup' H; [|exact Heq]; clear Heq.
       sep_rewrite_in mps_eq2_tup H; [|exact HP].
-      
 
       Lemma sh_spec_is_tup_array d n sh stk:
         stk ||= sh_spec (map (fun sv => (sv, n)) (locals sh d)) <=>
-            Ex f, is_tuple_array_p (map Sh (vars2es (locals sh d))) n f 0 1.
+            Ex f, (is_tuple_array_p (map Sh (vars2es (locals sh d))) n f 0 1).
       Proof.
         induction d; simpl; eauto.
         - split; intros.
-          + exists (fun _ : nat => @nil val); eauto.
-          + destruct H; eauto.
+          + exists (fun _ : nat => @nil val); sep_split; unfold_conn; eauto.
+          + destruct H; sep_split_in H; eauto.
         - simpl; rewrite IHd; split; intros H.
           + apply ex_lift_l_in in H as [f0 H].
             apply ex_lift_r_in in H as [f1 H].
@@ -1812,10 +1777,39 @@ Section Reduce.
             revert H; apply scRw; intros s h' H'; eauto.
             apply is_array_p1; eauto.
           + destruct H as [f H].
+            sep_split_in H.
             apply ex_lift_l; exists (fun x => hd 0%Z (f x)).
             apply scC, ex_lift_l; exists (fun x => tl (f x)).
             apply scC; revert H; apply scRw; intros s h' H'; eauto.
             apply is_array_p1 in H'; eauto.
+      Qed.
+
+      Lemma sh_spec_is_tup_array_with_l d n sh stk:
+        stk ||= sh_spec (map (fun sv => (sv, n)) (locals sh d)) <=>
+            Ex f, (is_tuple_array_p (map Sh (vars2es (locals sh d))) n f 0 1 **
+                   !(pure (forall i, length (f i) = d))).
+      Proof.
+        induction d; simpl; eauto.
+        - split; intros.
+          + exists (fun _ : nat => @nil val); sep_split; unfold_conn; eauto.
+          + destruct H; sep_split_in H; eauto.
+        - simpl; rewrite IHd; split; intros H.
+          + apply ex_lift_l_in in H as [f0 H].
+            apply ex_lift_r_in in H as [f1 H].
+            exists (fun x => f0 x :: f1 x); simpl.
+            sep_split; [|revert H; apply scRw; intros s h' H'; eauto].
+            2: apply is_array_p1; eauto.
+            sep_split_in H; unfold_conn_all; intros; rewrite HP; congruence.
+            sep_split_in H'; auto.
+          + destruct H as [f H].
+            sep_split_in H.
+            apply ex_lift_l; exists (fun x => hd 0%Z (f x)).
+            apply scC, ex_lift_l; exists (fun x => tl (f x)).
+            apply scC; revert H; apply scRw; intros s h' H'; eauto.
+            apply is_array_p1 in H'; eauto.
+            sep_split; eauto.
+            unfold_conn_all; simpl; intros.
+            lets: (HP i0); destruct (f i0); simpl in *; try omega.
       Qed.
       unfold sh_decl; sep_rewrite sh_spec_is_tup_array.
       apply ex_lift_l; exists (f (min (l - nf j * ntrd) ntrd) (f_seq g) e_b).
@@ -1829,9 +1823,12 @@ Section Reduce.
           congruence.
         - rewrite length_nseq; auto. } Unfocus.
       sep_normal; repeat sep_cancel.
-      revert H2; apply scRw; eauto; intros.
+      revert H2; apply scRw_stack; eauto; intros.
+      lets Heq : (Skel_lemma.mps_eq1_tup Outs' out); unfold es2gls in Heq; eauto.
+      sep_rewrite_in Heq H2; eauto.
+      (* sep_rewrite_in mps_eq1_tup *)
       eapply input_spec_forget; eauto.
-    - destruct Nat.eq_dec; try omega.
+    - destruct Nat.eq_dec; [clear HP6; unfold_pures; omega|].
       repeat sep_rewrite emp_unit_l.
       sep_rewrite_in emp_unit_l H; sep_rewrite_in emp_unit_r H.
       eapply input_spec_forget; eauto.
@@ -1889,5 +1886,304 @@ Section Reduce.
       apply (Var "").
       apply (Var "").
       apply (Var "").
+      apply (Var "").
+      apply (Var "").
+      apply (Var "").
+      apply (Var "").
+      apply (Var "").
+      apply (Var "").
+      apply (Var "").
+      apply (Var "").
+      apply (Var "").
+      apply (Var "").
+      apply (Var "").
+      apply (Var "").
+      apply (Var "").
+      apply (Var "").
+      apply (Var "").
+      apply (Var "").
+      apply (Var "").
+      apply (Var "").
+      apply (Var "").
+      apply (Var "").
+      apply (Var "").
+      apply (Var "").
+      apply (Var "").
+      apply (Var "").
+      apply (Var "").
+      apply (Var "").
+      apply (Var "").
+      apply (Var "").
+      apply (Var "").
+      apply (Var "").
+      apply (Var "").
+      apply (Var "").
+      apply (Var "").
+      apply (Var "").
   Qed.
+  End SeqReduce.
+
+  Definition bth_pre (j : Fin.t nblk) :=
+    !(sh === Zn l) ** !(Outs' ==t out) **
+    sh_spec sh_decl **
+    conj_xs (ls_init 0 ntrd (fun i => input_spec env env_den (perm_n nt_gr))) **
+    (map Gl Outs' +ol Zn (nf j) -->l (1, vs2es (fout (nf j)))).
+
+  Definition tr_pres (j : Fin.t nblk) := MyVector.init (fun i : Fin.t ntrd =>
+    Ex vi_ini, 
+      !(bid === Zn (nf j)) ** !(sh === Zn l) ** !(Outs' ==t out) ** !(pure (length vi_ini = dim)) **
+      (sdata' +ol Zn (nf i) -->l (1, vs2es vi_ini)) **
+      input_spec env env_den (perm_n nt_gr) **
+      if Nat.eq_dec (nf i) 0 then map Gl Outs' +ol Zn (nf j) -->l (1, vs2es (fout (nf j))) else emp).
+
+  Definition tr_posts g (j : Fin.t nblk) := MyVector.init (fun i : Fin.t ntrd =>
+    input_spec' env_den (perm_n nt_gr) **
+    (if Nat.eq_dec (nf i) 0 then sh_spec sh_decl else emp) **
+    (if Nat.eq_dec (nf i) 0 then
+       map Gl (vs2es out) +ol Zn (nf j) -->l
+           (1, vs2es (f (Nat.min (l - nf j * ntrd) ntrd) (f_seq j g) e_b 0))
+     else emp)).
+
+  Definition bth_post g (j : Fin.t nblk) := 
+    sh_spec sh_decl **
+    (map Gl (vs2es out) +ol Zn (nf j) -->l
+        (1, vs2es (f (Nat.min (l - nf j * ntrd) ntrd) (f_seq j g) e_b 0))) **
+    conj_xs (ls_init 0 ntrd (fun i => input_spec' env_den (perm_n nt_gr))).
+
+  Definition E (t : var) :=
+    if var_eq_dec t (Var "bid") then Lo
+    else if var_eq_dec t (Var "sh") then Lo
+    else if prefix "sdata" (var_of_str t) then Lo
+    else if prefix "Out" (var_of_str t) then Lo
+    else if prefix "sh" (var_of_str t) then Lo
+    else if prefix "arr" (var_of_str t) then Lo
+    else Hi.
+
+  Lemma read_tup_no_bars xs es : barriers (read_tup xs es) = nil.
+  Proof.
+    revert es; induction xs; destruct es; simpl; eauto.
+  Qed.
+
+  Ltac env_dec :=
+    repeat lazymatch goal with
+      | [|- context [prefix ?X ?Y]] => destruct (prefix X Y) eqn:?
+      | [|- context [var_eq_dec ?X ?Y]] => destruct (var_eq_dec X Y) eqn:?
+      end.
+    
+  Lemma reduce_aux_Lo a b : typing_cmd E (reduce_aux a b) Lo.
+  Proof.
+    revert a; induction b; simpl; constructor; eauto.
+    unfold E, reduce_body.
+    constructor; [constructor|].
+    repeat econstructor; repeat instantiate (1 := Hi); eauto; unfold join;
+      apply typing_cmd_Hi; try rewrite read_tup_no_bars; try rewrite gen_read_no_bars;
+        try rewrite gen_write_no_bars; auto;
+          try rewrite read_tup_writes; try rewrite writes_var_gen_write;
+            try rewrite gen_read_writes; try destruct var_eq_dec; subst;
+              intros; repeat destruct var_eq_dec; substs; simpl in *; try congruence; eauto;
+                (try now (forwards*: locals_pref; simpl in *; congruence));
+                (try now (forwards * : func_local; simpl in *; congruence));
+                (try now (unfold vars2es; repeat rewrite map_length; repeat rewrite locals_length;
+                         repeat rewrite get_wf; repeat rewrite func_wf; eauto));
+                env_dec; eauto; simplify; simpl; try congruence;
+    forwards* : func_local; simpl in *; congruence.
+    Grab Existential Variables.
+    apply 1.
+    apply "".
+    apply (Var "").
+    apply 1.
+    apply "".
+    apply (Var "").
+    apply 1.
+    apply "".
+    apply (Var "").
+  Qed.
+ 
+  Lemma fold_has_type : typing_cmd E mkFoldAll Lo.
+  Proof.
+    unfold mkFoldAll, seq_reduce, reduce, setToLen, E.
+    repeat constructor.
+    - eapply weaken_type; try apply read_tup_hi; eauto.
+      intros; env_dec; simplify; try congruence.
+    - eapply weaken_type; try apply typing_cmd_Hi; eauto.
+      + apply gen_write_no_bars.
+      + intros; rewrite writes_var_gen_write in H; simpl in *; tauto.
+    - econstructor; repeat constructor; simpl.
+      instantiate (1 := Hi); eauto.
+      repeat instantiate (1 := Hi); eauto.
+    - eapply weaken_type; try apply typing_cmd_Hi; eauto; simpl.
+      + rewrite get_no_bar, func_no_bars, !read_tup_no_bars, gen_write_no_bars; eauto.
+      + rewrite !read_tup_writes;
+        try now (unfold vars2es; repeat rewrite map_length; repeat rewrite locals_length;
+                 repeat rewrite get_wf; repeat rewrite func_wf; eauto).
+        rewrite !writes_var_gen_write;
+        intros; env_dec; substs;
+        repeat (rewrite in_app_iff in H; simpl in H);
+        simplify; try congruence;
+        (try now (forwards*: get_wr; eauto; simplify; simpl in *; congruence));
+        (try now (forwards*: func_local; eauto; simplify; simpl in *; congruence)).
+    - eapply weaken_type; try apply typing_cmd_Hi; simpl; eauto.
+      intros; simplify; eauto; destruct var_eq_dec; congruence.
+    - apply reduce_aux_Lo.
+    - applys (>>weaken_type Hi); eauto.
+      apply typing_cmd_Hi; simpl; eauto.
+      rewrite gen_read_no_bars, gen_write_no_bars; auto.
+      rewrite gen_read_writes, writes_var_gen_write; simpl.
+      intros; repeat rewrite in_app_iff in H;
+        env_dec; substs; simplify; congruence.
+      unfold vars2es; rewrite map_length, !locals_length; auto.
+      Grab Existential Variables.
+      apply (Var "").
+      apply (Var "").
+      apply (Var "").
+      apply (Var "").
+      apply (Var "").
+      apply (Var "").
+      apply (Var "").
+      apply (Var "").
+  Qed.
+
+  Lemma prefix_nil s : prefix "" s = true. destruct s; eauto. Qed.
+  Notation skip_sum_of_vs := (skip_sum_of_opt (list val) f_fun).
+
+  Lemma reduce_ok_bl g (j : Fin.t nblk) :
+    (forall i, i < l -> get_den (Zn i) (g i)) ->
+    CSLp ntrd E
+         (!(bid === Zn (nf j)) ** bth_pre j)
+         mkFoldAll 
+         (bth_post g j).
+  Proof.
+    intros Hg.
+    applys (>> rule_par (BS' j g) (tr_pres j) (tr_posts g j)).
+    - destruct ntrd; try omega; eexists; eauto.
+    - intros; split; intros;
+      unfold BS', BS, BSpre, BSpost, Binv, E, CSL.low_assn; simpl;
+      rewrite MyVector.init_spec; simpl;
+      destruct i; repeat prove_low_assn;
+        (try now (first [apply low_assn_is_tuple|apply low_assn_is_tup_arr]; simplify; repeat econstructor;
+                  cutrewrite (Lo = join Lo Lo); [|auto]; repeat econstructor; simpl;
+                  rewrite prefix_nil; auto)).
+    - unfold BS'; intros; apply BS_ok; eauto.
+      rewrite Nat.le_min_r; auto.
+      intros; unfold f_seq, maybe; destruct (skip_sum_of_vs _ _ _ _ _) eqn:Heq.
+      + erewrite skip_sum_of_vs_wf; eauto.
+        intros ix ?; forwards * : (>>get_den_wf (Zn ix)); rewrite out_wf.
+        congruence.
+      + rewrite length_nseq; auto.
+    - Lemma precise_pts : forall (e1 : loc_exp) (e2 : exp) (q : Qc), precise (e1 -->p (q,  e2)).
+      Proof.
+        intros; unfold precise; simpl; intros; unfold_conn_all.
+        destruct h1, h1'; apply pheap_eq; extensionality x; simpl in *.
+        rewrite H, H0; destruct (eq_dec _ _); eauto.
+      Qed.
+
+      Lemma is_tup_precise E q v : precise (E -->l (q, v)).
+      Proof.
+        revert v; induction E; simpl; destruct v; eauto using precise_emp.
+        apply precise_star; eauto using precise_pts.
+      Qed.
+      
+      Lemma precise_is_array_p e len s f' p : precise (is_array_p e len f' s p).
+      Proof.
+        revert s; induction len; simpl; intros; eauto using precise_emp, precise_star, precise_pts.
+      Qed.  
+
+      Lemma is_tup_arr_precise E len f s q  : precise (is_tuple_array_p E len f s q).
+      Proof.
+        revert f; induction E; simpl; eauto using precise_emp.
+        intros f; eauto using precise_star, precise_is_array_p.
+      Qed.
+        
+      split; unfold BS', BS, BSpre, BSpost, Binv; simpl; rewrite MyVector.init_spec;
+        destruct i; repeat destruct Sumbool.sumbool_and; repeat destruct Nat.eq_dec;
+      repeat apply precise_star; eauto using precise_emp, is_tup_precise, is_tup_arr_precise.
+
+    - unfold bth_pre, tr_pres; intros; istar_simplify.
+      sep_rewrite (@ls_exists0 _ (ls_init 0 dim (fun i => 0%Z))).
+      unfold sh_decl in H.
+      sep_rewrite_in sh_spec_is_tup_array_with_l H.
+      sep_split_in H.
+      apply ex_lift_l_in in H as [f_sm H].
+      sep_normal_in H; sep_split_in H.
+      exists (ls_init 0 ntrd f_sm).
+      sep_split; [unfold_conn; simpl; rewrite init_length; auto|].
+      repeat sep_rewrite (@ls_star); repeat sep_rewrite (@ls_pure); sep_split.
+      apply ls_emp'; intros; rewrite ls_init_spec; destruct lt_dec; eauto; cbv; auto.
+      apply ls_emp'; intros; rewrite ls_init_spec; destruct lt_dec; eauto; cbv; auto.
+      apply ls_emp'; intros; rewrite ls_init_spec; destruct lt_dec; eauto; cbv; auto.
+      apply ls_emp'; intros; rewrite ls_init_spec; destruct lt_dec; unfold_conn; eauto;[| cbv; auto].
+      rewrite ls_init_spec; destruct lt_dec; try omega; unfold_conn_in HP2; rewrite HP2; auto.
+      sep_cancel.
+      sep_rewrite is_tuple_array_p_distr; sep_cancel.
+      2: intros; rewrite ls_init_spec; destruct lt_dec; try rewrite init_length.
+      2: unfold_conn_in HP2; unfold vars2es; rewrite HP2, !map_length, !locals_length; auto.
+      2: unfold vars2es; rewrite !map_length, locals_length; auto.
+      2: instantiate (1 := nseq dim 0%Z); rewrite length_nseq; auto.
+      apply scC; rewrite <-(@firstn_skipn assn 1) at 1; rewrite firstn_init, skipn_init.
+      rewrite Nat.min_l; try omega; simpl; sep_normal.
+      erewrite ls_init_eq'.
+      2: intros; destruct Nat.eq_dec; try omega;
+        cutrewrite (emp = id (fun _ => emp) (1 + i)); eauto.
+      unfold id; sep_rewrite init_emp_emp.
+      sep_rewrite emp_unit_l; sep_normal.
+      sep_cancel.
+      eapply is_tup_array_change; eauto.
+      intros; rewrite ls_init_spec; destruct lt_dec; try omega; f_equal; omega.
+    - (* not completed!!!! *)
+      unfold tr_posts, bth_post; intros s h H; istar_simplify_in H.
+      rewrite <-(firstn_skipn 1) in H at 1; rewrite firstn_init, skipn_init in H.
+      rewrite Nat.min_l in H; try omega; simpl in H.
+      erewrite (@ls_init_eq' _ _ _ _ 1) in H.
+      2: intros; destruct Nat.eq_dec; try omega;
+        cutrewrite (emp = id (fun _ => emp) (1 + i)); eauto.
+      unfold id in H; sep_rewrite_in init_emp_emp H.
+      apply scC in H; rewrite <-(firstn_skipn 1) in H at 1; rewrite firstn_init, skipn_init in H.
+      rewrite Nat.min_l in H; try omega; simpl in H.
+      erewrite ls_init_eq' in H.
+      2: intros; destruct Nat.eq_dec; try omega;
+        cutrewrite (emp = id (fun _ => emp) (1 + i)); eauto.
+      unfold id in H; sep_rewrite_in init_emp_emp H.
+      sep_normal_in H; repeat sep_cancel.
+      
+    - intros; unfold low_assn, tr_pres; rewrite MyVector.init_spec.
+      unfold E; repeat prove_low_assn;
+        (try now (constructor; eauto));
+        try now (unfold Outs; first [apply low_assn_eqt | apply low_assn_is_tuple];
+                 simplify; cutrewrite (Lo = join Lo Lo); repeat econstructor; simpl;
+                 try rewrite prefix_nil; auto).
+      apply low_assn_input_spec;
+      intros; env_dec; simplify; simpl in *; congruence.
+    - intros; unfold low_assn, tr_posts; rewrite MyVector.init_spec.
+      unfold E, sh_decl; simpl.
+      repeat prove_low_assn;
+        (try now (constructor; eauto));
+        try now (unfold Outs; first [apply low_assn_eqt | apply low_assn_is_tuple];
+                 simplify; cutrewrite (Lo = join Lo Lo); repeat econstructor; simpl;
+                 try rewrite prefix_nil; auto).
+
+      Lemma sh_spec_low_assn E sdec :
+        (forall x y, In (x, y) sdec -> E x = Lo) -> low_assn E (sh_spec sdec).
+      Proof.
+        intros.
+        induction sdec as [|[? ?] ?]; simpl; unfold low_assn; repeat prove_low_assn.
+        repeat constructor; erewrite H; eauto.
+        simpl; eauto.
+        apply IHsdec; simpl in H; eauto.
+      Qed.
+      apply sh_spec_low_assn; simplify; inverts H; simpl; rewrite prefix_nil; auto.
+      apply low_assn_input_spec'.
+    - apply fold_has_type.
+    - unfold tr_pres, tr_posts; intros; rewrite !MyVector.init_spec.
+      eapply Hbackward.
+      Focus 2. {
+        intros; apply ex_lift_l_in in H as [? H].
+        sep_normal_in H.
+        evar (P : assn); assert ((!(pure (Datatypes.length x = dim)) ** P) s0 h) by
+                           (sep_cancel; unfold P; eauto).
+        unfold P in *; ex_intro x H0; eauto. } Unfocus.
+      apply rule_ex; intros vi_ini.
+      apply hback; intros Hvini.
+      eapply rule_conseq; try apply (reduce_ok_th tid j vi_ini); intros; eauto; repeat sep_cancel.
+  Qed.
+
 End Reduce.
